@prefix : <http://sibils.org/rdf#> .
@prefix owl: <http://www.w3.org/2002/07/owl#> .
@prefix rdf: <http://www.w3.org/1999/02/22-rdf-syntax-ns#> .
@prefix rdfs: <http://www.w3.org/2000/01/rdf-schema#> .
@prefix dc: <http://purl.org/dc/elements/1.1/> .
@prefix xsd: <http://www.w3.org/2001/XMLSchema#> .
@prefix dct: <http://purl.org/dc/terms/> .
@prefix sdo: <https://schema.org/> .

@prefix skos: <http://www.w3.org/2004/02/skos/core#> .
@prefix deo: <http://purl.org/spar/deo/> .
@prefix doco: <http://purl.org/spar/doco/> .
@prefix fabio: <http://purl.org/spar/fabio/> .
@prefix po: <http://www.essepuntato.it/2008/12/pattern#> .

# @prefix openbiodiv: http://openbiodiv.net/> .

@prefix foaf: <http://xmlns.com/foaf/0.1/> .
@prefix prism: <http://prismstandard.org/namespaces/basic/2.0/> .
@prefix frbr: <http://purl.org/vocab/frbr/core#> .
@prefix oa: <http://www.w3.org/ns/oa#> .
@prefix cnt: <http://www.w3.org/2011/content#> .

<http://sibils.org/rdf> 
  a owl:Ontology ;
  owl:imports po: , deo: , doco: , fabio: , skos: ;
  dct:description "The SIBiLS ontology is used to represent annotated scientific publications";
  dct:created "2022-11-01"^^xsd:date ;
#  dct:creator [ 
#    a sdo:Person ;
#    sdo:affiliation <https://www.sib.swiss> ;
#    sdo:email "pierre-andre.michel@sib.swiss" ;
#    sdo:identifier <https://orcid.org/0000-0002-8742-7730> ;
#    sdo:name "Pierre-Andr√© Michel"
#  ] ;
  dct:license <http://creativecommons.org/licenses/by/4.0> ;
  dct:modified "2022-11-01"^^xsd:date ;
  dct:title "SIBiLS ontology" ;
  owl:versionInfo "Current release"^^xsd:string ;
  .
# ------------------------------------------------------

# Subclasses of https://sparontologies.github.io/deo/current/deo.html

:DiscourseElement
      rdf:type owl:Class ;
      rdfs:label "Discourse element"^^xsd:string;
      rdfs:comment "An element of a document that carries out a rhetorical function."^^xsd:string ;
      rdfs:subClassOf deo:DiscourseElement ;
      rdfs:isDefinedBy <http://sibils.org/rdf> ;
      .

:Caption
      rdf:type owl:Class ;
      rdfs:label "Caption"^^xsd:string;
      rdfs:comment "Caption of a text box."^^xsd:string ;
      rdfs:subClassOf :DiscourseElement, deo:Caption ;
      rdfs:isDefinedBy <http://sibils.org/rdf> ;
      .

# Subclasses of https://sparontologies.github.io/doco/current/doco.html

:Abstract
      rdf:type owl:Class ;
      rdfs:label "Abstract"^^xsd:string ;
      rdfs:comment "A brief summary of a book, a research article, thesis, review, conference proceeding or any in-depth analysis of a particular subject or discipline, the purpose of which is to help the reader quickly ascertain the publication's purpose."^^xsd:string ;
      rdfs:subClassOf :DiscourseElement, doco:Abstract ;
      rdfs:isDefinedBy <http://sibils.org/rdf> ;
      .

:Appendix
      rdf:type owl:Class ;
      rdfs:label "Appendix"^^xsd:string ;
      rdfs:comment "A supplemental addition to the main work. It may contain data, more detailed information about methods and materials, or provide additional detail concerning the information found in the main work."^^xsd:string ;
      rdfs:subClassOf :DiscourseElement, doco:Appendix ;
      rdfs:isDefinedBy <http://sibils.org/rdf> ;
      .

:BackMatter
      rdf:type owl:Class ;
      rdfs:label "Back matter"^^xsd:string ;
      rdfs:comment "The final principle part of a document, in which is usually found the bibliography, index, appendixes, etc."^^xsd:string ;
      rdfs:subClassOf :DiscourseElement, doco:BackMatter ;
      rdfs:isDefinedBy <http://sibils.org/rdf> ;
      .

:BlockQuotation
      rdf:type owl:Class ;
      rdfs:label "Block quotation"^^xsd:string ;
      rdfs:comment "A block quotation (also known as a long quotation or extract) is a quotation in a written document which is set off from the main text as a container for distinct paragraphs, which is typically distinguished visually using indentation, a different font, or smaller size. Block quotations are used for longer passages than run-in quotations (which are set off with quotation marks)."^^xsd:string ;
      rdfs:subClassOf :DiscourseElement, doco:BlockQuotation ;
      rdfs:isDefinedBy <http://sibils.org/rdf> ;
      .

:BodyMatter
      rdf:type owl:Class ;
      rdfs:label "Body matter"^^xsd:string ;
      rdfs:comment "The central principle part of a document, that contains the real content. It may be subdivided hierarchically by the use of chapters and sections."^^xsd:string ;
      rdfs:subClassOf :DiscourseElement, doco:BodyMatter ;
      rdfs:isDefinedBy <http://sibils.org/rdf> ;
      .

:CaptionedBox
      rdf:type owl:Class ;
      rdfs:label "Captioned box"^^xsd:string ;
      rdfs:comment "A rectangle space within a page that contains an object and its related caption."^^xsd:string ;
      rdfs:subClassOf :DiscourseElement, doco:CaptionedBox ;
      rdfs:isDefinedBy <http://sibils.org/rdf> ;
      .

:FigureBox
      rdf:type owl:Class ;
      rdfs:label "Figure box"^^xsd:string ;
      rdfs:comment "A space within a document that contains a figure and its caption."^^xsd:string ;
      rdfs:subClassOf :DiscourseElement, doco:FigureBox ;
      rdfs:isDefinedBy <http://sibils.org/rdf> ;
      .

:FloatMatter
      rdf:type owl:Class ;
      rdfs:label "Float matter"^^xsd:string ;
      rdfs:comment "Floating part of a document related to some aspect of the body section. Usually in a box with its own body with some title and / or caption."^^xsd:string ;
      rdfs:subClassOf :DiscourseElement ;
      rdfs:isDefinedBy <http://sibils.org/rdf> ;
      .

:FrontMatter
      rdf:type owl:Class ;
      rdfs:label "Front matter"^^xsd:string ;
      rdfs:comment "The initial principle part of a document, usually containing self-referential metadata. In a book, this typically includes its title, authors, publisher, publication date, ISBN and copyright declaration, together with the preface, foreword, table of content, etc. In a journal article, the front matter is normally restricted to the title, authors and the authors' affiliation details, although the latter may alternatively be included in a footnote or the back matter. In books, the front matter pages may be numbered in lowercase Roman numerals."^^xsd:string ;
      rdfs:subClassOf :DiscourseElement, doco:FrontMatter ;
      rdfs:isDefinedBy <http://sibils.org/rdf> ;
      .

:Glossary
      rdf:type owl:Class ;
      rdfs:label "Glossary"^^xsd:string ;
      rdfs:comment "A set of definitions of words or phrases of importance to the work, normally alphabetized. In longer works of fiction, the entries may contains places and characters."^^xsd:string ;
      rdfs:subClassOf :DiscourseElement, doco:Glossary ;
      rdfs:isDefinedBy <http://sibils.org/rdf> ;
      .

:Label
      rdf:type owl:Class ;
      rdfs:label "Label"^^xsd:string ;
      rdfs:comment """A block containing text, that may include a number (e.g., "Chapter Three", "3.2", "Figure 1", "Table"), used to identify an item within the document, for example a chapter, a figure, a section or a table."""^^xsd:string ;
      rdfs:subClassOf :DiscourseElement, doco:Label ;
      rdfs:isDefinedBy <http://sibils.org/rdf> ;
      .

:ListItemBlock
      rdf:type owl:Class ;
      rdfs:label "List item block"^^xsd:string ;
      rdfs:comment "A list item part of a document. Usually appears multiple time in a sequence. May be prefixed with a bullet or a number."^^xsd:string ;
      rdfs:subClassOf :DiscourseElement ;
      rdfs:isDefinedBy <http://sibils.org/rdf> ;
      .

:ListOfReferences
      rdf:type owl:Class ;
      rdfs:label "List of references"^^xsd:string ;
      rdfs:comment "A list of items each representing a reference to a specific part of the same document, or to another publication."^^xsd:string ;
      rdfs:subClassOf :DiscourseElement, doco:ListOfReferences ;
      rdfs:isDefinedBy <http://sibils.org/rdf> ;
      .

:MediaBlock
      rdf:type owl:Class ;
      rdfs:label "Media block"^^xsd:string ;
      rdfs:comment "A reference or link to some media (audio, video) part of a document."^^xsd:string ;
      rdfs:subClassOf :DiscourseElement ;
      rdfs:isDefinedBy <http://sibils.org/rdf> ;
      .

:ObjectIdBlock
      rdf:type owl:Class ;
      rdfs:label "Object id block"^^xsd:string ;
      rdfs:comment "An identifier appearing as a distinct part of a document."^^xsd:string ;
      rdfs:subClassOf :DiscourseElement ;
      rdfs:isDefinedBy <http://sibils.org/rdf> ;
      .

:Paragraph
      rdf:type owl:Class ;
      rdfs:label "Paragraph"^^xsd:string ;
      rdfs:comment "A self-contained unit of discourse that deals with a particular point or idea. Paragraphs contains one or more sentences. The start of a paragraph is indicated by beginning on a new line, which may be indented or separated by a small vertical space by the preceding paragraph."^^xsd:string ;
      rdfs:subClassOf :DiscourseElement, doco:Paragraph ;
      rdfs:isDefinedBy <http://sibils.org/rdf> ;
      .

:Section
      rdf:type owl:Class ;
      rdfs:label "Section"^^xsd:string ;
      rdfs:comment "A logical division of the text, usually numbered and/or titled, which may contain subsections."^^xsd:string ;
      rdfs:subClassOf :DiscourseElement, doco:Section ;
      rdfs:isDefinedBy <http://sibils.org/rdf> ;
      .

:SectionLabel
      rdf:type owl:Class ;
      rdfs:label "Section label"^^xsd:string ;
      rdfs:comment "A block containing a label for the section, that may include the section number."^^xsd:string ;
      rdfs:subClassOf :DiscourseElement, doco:SectionLabel ;
      rdfs:isDefinedBy <http://sibils.org/rdf> ;
      .

:SpeechBlock
      rdf:type owl:Class ;
      rdfs:label "Speech block"^^xsd:string ;
      rdfs:comment "A dialog or part of dialog appearing as a distinct part of a document."^^xsd:string ;
      rdfs:subClassOf :DiscourseElement ;
      rdfs:isDefinedBy <http://sibils.org/rdf> ;
      .


:StatementBlock
      rdf:type owl:Class ;
      rdfs:label "Statement block"^^xsd:string ;
      rdfs:comment "A statement appearing as a distinct part of a document."^^xsd:string ;
      rdfs:subClassOf :DiscourseElement ;
      rdfs:isDefinedBy <http://sibils.org/rdf> ;
      .

:Table
      rdf:type owl:Class ;
      rdfs:label "Table"^^xsd:string ;
      rdfs:comment "A set of data arranged in cells within rows and columns."^^xsd:string ;
      rdfs:subClassOf :DiscourseElement, doco:Table ;
      rdfs:isDefinedBy <http://sibils.org/rdf> ;
      .

:TableBox
      rdf:type owl:Class ;
      rdfs:label "Table box"^^xsd:string ;
      rdfs:comment "A space within a document that contains a table and its caption."^^xsd:string ;
      rdfs:subClassOf :DiscourseElement, doco:TableBox ;
      rdfs:isDefinedBy <http://sibils.org/rdf> ;
      .

:TextBox
      rdf:type owl:Class ;
      rdfs:label "Text box"^^xsd:string ;
      rdfs:comment "A space within a document that contains textual content relating to, quoting from or expanding upon the main text. Usually a textbox is delimited by a border or use of a background colour distinct from that of the main text."^^xsd:string ;
      rdfs:subClassOf :DiscourseElement, doco:TextBox ;
      rdfs:isDefinedBy <http://sibils.org/rdf> ;
      .

:Title
      rdf:type owl:Class ;
      rdfs:label "Title"^^xsd:string ;
      rdfs:comment "A word, phrase or sentence that precedes and indicates the subject of a document or a document component - e.g., a book, a report, a news article, a chapter, a section or a table."^^xsd:string ;
      rdfs:subClassOf :DiscourseElement, doco:Title ;
      rdfs:isDefinedBy <http://sibils.org/rdf> ;
      .

:VerseGroupBlock
      rdf:type owl:Class ;
      rdfs:label "Verse group block"^^xsd:string ;
      rdfs:comment "A block containing one or several verses appearing as a distinct part of a document."^^xsd:string ;
      rdfs:subClassOf :DiscourseElement ;
      rdfs:isDefinedBy <http://sibils.org/rdf> ;
      .


# Suclasses of https://sparontologies.github.io/fabio/current/fabio.html


:Publication
      rdf:type owl:Class ;
      rdfs:label "Publication"^^xsd:string ;
      rdfs:comment "A subclass of fabio expression, restricted to publications in SIBiLS."^^xsd:string ;
      rdfs:subClassOf fabio:Expression ;
      rdfs:isDefinedBy <http://sibils.org/rdf> ;
      .

:BriefReport
      rdf:type owl:Class ;
      rdfs:label "Brief report"^^xsd:string ;
      rdfs:comment "A brief report document. This term may also be used synonymously with Rapid Communication to mean 'A short rapidly published research article or conference paper, typically reporting significant research results that have been recently discovered, or a brief news item reporting such discoveries.'"^^xsd:string ;
      rdfs:subClassOf :Publication, fabio:BriefReport ;
      rdfs:isDefinedBy <http://sibils.org/rdf> ;
      .

:CaseReport
      rdf:type owl:Class ;
      rdfs:label "Case report"^^xsd:string ;
      rdfs:comment "A report about a particular case or situation."^^xsd:string ;
      rdfs:subClassOf :Publication, fabio:CaseReport ;
      rdfs:isDefinedBy <http://sibils.org/rdf> ;
      .

:Editorial
      rdf:type owl:Class ;
      rdfs:label "Editorial"^^xsd:string ;
      rdfs:comment "The realization of an opinion written by an editor."^^xsd:string ;
      rdfs:subClassOf :Publication, fabio:Editorial ;
      rdfs:isDefinedBy <http://sibils.org/rdf> ;
      .

:JournalArticle
      rdf:type owl:Class ;
      rdfs:label "Journal article"^^xsd:string ;
      rdfs:comment "An article, typically the realization of a research paper reporting original research findings, published in a journal issue."^^xsd:string ;
      rdfs:subClassOf :Publication, fabio: ;
      rdfs:isDefinedBy <http://sibils.org/rdf> ;
      .

:Letter
      rdf:type owl:Class ;
      rdfs:label "Letter"^^xsd:string ;
      rdfs:comment "A written or printed communication of a personal or professional nature between individuals and/or representatives of corporate bodies, usually transmitted by the postal service or published in a periodical. In the latter case, the letter is typically addressed to the editor and comments on or discussed an item previously published by that periodical, or of interest to its readership."^^xsd:string ;
      rdfs:subClassOf :Publication, fabio:JournalArticle ;
      rdfs:isDefinedBy <http://sibils.org/rdf> ;
      .

:MeetingReport
      rdf:type owl:Class ;
      rdfs:label "Meeting report"^^xsd:string ;
      rdfs:comment "A report of a meeting of some kind."^^xsd:string ;
      rdfs:subClassOf :Publication, fabio:MeetingReport ;
      rdfs:isDefinedBy <http://sibils.org/rdf> ;
      .

:ReviewArticle
      rdf:type owl:Class ;
      rdfs:label "Review article"^^xsd:string ;
      rdfs:comment "An article that contains a review."^^xsd:string ;
      rdfs:subClassOf :Publication, fabio:ReviewArticle ;
      rdfs:isDefinedBy <http://sibils.org/rdf> ;
      .


:Manifestation
      rdf:type owl:Class ;
      rdfs:label "Manifestation"^^xsd:string ;
      rdfs:comment "A subclass of fabio manifestation. Specifically applies to electronic (digital) as well as to physical manifestations of expressions."^^xsd:string ;
      rdfs:subClassOf fabio:Manifestation ;
      rdfs:isDefinedBy <http://sibils.org/rdf> ;
      .

# Classes dereived from http://www.essepuntato.it/2008/12/pattern#Block

# TODO flag parts as subc class of block ?
:Block
      rdf:type owl:Class ;
      rdfs:label "Block"^^xsd:string ;
      rdfs:comment ""^^xsd:string ;
      rdfs:subClassOf po:Block ;
      rdfs:isDefinedBy <http://sibils.org/rdf> ;
      .

# Properties (derived) found in http://openbiodiv.net/

# NOTE: can't find where it is defined in openbiodiv ontology
# See https://github.com/pensoft/OpenBiodiv/blob/master/ontology/openbiodiv-ontology.ttl

:affiliation a rdf:Property, owl:DatatypeProperty ;
      rdfs:label "affiliation"^^xsd:string ;
      rdfs:comment "Links a person, usually an author, to an organization they are affiliated to."^^xsd:string ;
      rdfs:domain foaf:Person ;
      rdfs:range xsd:string ;
      rdfs:isDefinedBy <http://sibils.org/rdf> ;
      .

# NOTE: in openbiodiv :contains is just a sublass of po:contains, no more semantic
# so it is better to define our own 

:contains rdf:type owl:ObjectProperty, owl:TransitiveProperty ;
      rdfs:subPropertyOf po:contains ;
      rdfs:label "contains"^^xsd:string ;
      rdfs:comment "Relationships between a discourse element containing another one."^^xsd:string ;
      rdfs:domain :DiscourseElement ;
      rdfs:range :DiscourseElement ;
      rdfs:isDefinedBy <http://sibils.org/rdf> ;
      .


# Properties derived fro prism http://prismstandard.org/namespaces/basic/2.0/
# NOTE: the definition are inspired of what is found in fabio : 
# See https://sparontologies.github.io/fabio/current/fabio.html

:doi a rdf:Property, owl:DatatypeProperty ;
      rdfs:subPropertyOf prism:doi ;
      rdfs:label "doi"^^xsd:string ;
      rdfs:comment "Links a publication to its Digital Object Identifier."^^xsd:string ;
      rdfs:domain :Publication ;
      rdfs:range xsd:string ;
      rdfs:isDefinedBy <http://sibils.org/rdf> ;
      .

:endingPage a rdf:Property, owl:DatatypeProperty ;
      rdfs:subPropertyOf prism:endingPage ;
      rdfs:label "ending page"^^xsd:string ;
      rdfs:comment "Links a publication to the last page of the journal containing it."^^xsd:string ;
      rdfs:domain :Publication ;
      rdfs:range xsd:string ;
      rdfs:isDefinedBy <http://sibils.org/rdf> ;
      .

:issueIdentifier a rdf:Property, owl:DatatypeProperty ;
      rdfs:subPropertyOf prism:issueIdentifier ;
      rdfs:label "issue identifier page"^^xsd:string ;
      rdfs:comment "Links a publication to an identifier used to identify a specific issue of a magazine, a journal or other resource."^^xsd:string ;
      rdfs:domain :Publication ;
      rdfs:range xsd:string ;
      rdfs:isDefinedBy <http://sibils.org/rdf> ;
      .

:keyword a rdf:Property, owl:DatatypeProperty ;
      rdfs:subPropertyOf prism:endingkeywordPage ;
      rdfs:label "keyword"^^xsd:string ;
      rdfs:comment "Links a publication with a keyword that is likely to be used in search queries."^^xsd:string ;
      rdfs:domain :Publication ;
      rdfs:range xsd:string ;
      rdfs:isDefinedBy <http://sibils.org/rdf> ;
      .

:pageRange a rdf:Property, owl:DatatypeProperty ;
      rdfs:subPropertyOf prism:pageRange ;
      rdfs:label "page range"^^xsd:string ;
      rdfs:comment "Links a publication to the pages of a journal where it appears."^^xsd:string ;
      rdfs:domain :Publication ;
      rdfs:range xsd:string ;
      rdfs:isDefinedBy <http://sibils.org/rdf> ;
      .

:publicationDate a rdf:Property, owl:DatatypeProperty ;
      rdfs:subPropertyOf prism:publicationDate ;
      rdfs:label "publication date"^^xsd:string ;
      rdfs:comment "Links a publication to its publication date."^^xsd:string ;
      rdfs:domain :Publication ;
      rdfs:range xsd:date ;
      rdfs:isDefinedBy <http://sibils.org/rdf> ;
      .

:startingPage a rdf:Property, owl:DatatypeProperty ;
      rdfs:subPropertyOf prism:startingPage ;
      rdfs:label "starting page"^^xsd:string ;
      rdfs:comment "Links a publication to the first page of the journal containing it"^^xsd:string ;
      rdfs:domain :Publication ;
      rdfs:range xsd:string ;
      rdfs:isDefinedBy <http://sibils.org/rdf> ;
      .

:volume a rdf:Property, owl:DatatypeProperty ;
      rdfs:subPropertyOf prism:volume ;
      rdfs:label "volume"^^xsd:string ;
      rdfs:comment "Links a publication to an identifier for a particular volume of a resource, such as a journal or a multi-volume book."^^xsd:string ;
      rdfs:domain :Publication ;
      rdfs:range xsd:string ;
      rdfs:isDefinedBy <http://sibils.org/rdf> ;
      .

# Properties derived from dct http://purl.org/dc/terms/

:abstract a rdf:Property, owl:DatatypeProperty ;
      rdfs:subPropertyOf dct:abstract ;
      rdfs:label "abstract"^^xsd:string ;
      rdfs:comment "Links a publication to  its abstract as a string."^^xsd:string ;
      rdfs:domain :Publication ;
      rdfs:range xsd:string ;
      rdfs:isDefinedBy <http://sibils.org/rdf> ;
      .

:creator a rdf:Property, owl:ObjectProperty ;
      rdfs:subPropertyOf dct:creator ;
      rdfs:label "creator"^^xsd:string ;
      rdfs:comment "Links a publication to a person involved in its creation."^^xsd:string ;
      rdfs:domain :Publication ;
      rdfs:range foaf:Person ;
      rdfs:isDefinedBy <http://sibils.org/rdf> ;
      .

:title a rdf:Property, owl:DatatypeProperty ;
      rdfs:subPropertyOf dct:title ;
      rdfs:label "title"^^xsd:string ;
      rdfs:comment "Links a publication to its title."^^xsd:string ;
      rdfs:domain :Publication ;
      rdfs:range xsd:string ;
      rdfs:isDefinedBy <http://sibils.org/rdf> ;
      .

# Properties derived from fabio ontology http://purl.org/spar/fabio

:hasNLMJournalTitleAbbreviation a rdf:Property, owl:DatatypeProperty ;
      rdfs:subPropertyOf fabio:hasNLMJournalTitleAbbreviation ;
      rdfs:label "has NLM journal title abbreviation"^^xsd:string ;
      rdfs:comment "Links a publication to an internal identifier for the abbreviation of the title of journals available from the National Library of Medicine repositoryn."^^xsd:string ;
      rdfs:domain :Publication ;
      rdfs:range xsd:string ;
      rdfs:isDefinedBy <http://sibils.org/rdf> ;
      .

:hasPubMedCentralId a rdf:Property, owl:DatatypeProperty ;
      rdfs:subPropertyOf fabio:hasPubMedCentralId ;
      rdfs:label "has PubMed Central id"^^xsd:string ;
      rdfs:comment "Links a publication to an identifier for bibliographic entities hosted by the PubMed Central repository."^^xsd:string ;
      rdfs:domain :Publication ;
      rdfs:range xsd:string ;
      rdfs:isDefinedBy <http://sibils.org/rdf> ;
      .

:hasPubMedId a rdf:Property, owl:DatatypeProperty ;
      rdfs:subPropertyOf fabio:hasPubMedId ;
      rdfs:label "has PubMed id"^^xsd:string ;
      rdfs:comment "Links a publication to an identifier for bibliographic records held by the PubMed repository."^^xsd:string ;
      rdfs:domain :Publication ;
      rdfs:range xsd:string ;
      rdfs:isDefinedBy <http://sibils.org/rdf> ;
      .

:hasPublicationYear a rdf:Property, owl:DatatypeProperty ;
      rdfs:subPropertyOf fabio:hasPublicationYear ;
      rdfs:label "has publication year"^^xsd:string ;
      rdfs:comment "Links a publication to the year in which it was published."^^xsd:string ;
      rdfs:domain :Publication ;
      rdfs:range xsd:integer ;
      rdfs:isDefinedBy <http://sibils.org/rdf> ;
      .


# Properties derived from frbr http://purl.org/vocab/frbr/core#

:embodiment a rdf:Property, owl:ObjectProperty ;
      rdfs:subPropertyOf frbr:embodiment ;
      rdfs:label "embodiment"^^xsd:string ;
      rdfs:comment "Links a publication to its manifestation."^^xsd:string ;
      rdfs:domain :Publication ;
      rdfs:range :Manifestation ;
      rdfs:isDefinedBy <http://sibils.org/rdf> ;
      .

# Classes and Properties related and / or derived from oa http://www.w3.org/ns/oa#

:Annotation
      rdf:type owl:Class ;
      rdfs:label "Annotation"^^xsd:string ;
      rdfs:comment "A concept identified at a specific position in a discourse element of a publication by a named entity extraction process."^^xsd:string ;
      rdfs:subClassOf oa:Annotation ;
      rdfs:isDefinedBy <http://sibils.org/rdf> ;
      .

:AnnotationTarget
      rdf:type owl:Class ;
      rdfs:label "Annotation target"^^xsd:string ;
      rdfs:comment "Location of the annotation in a discourse element."^^xsd:string ;
      rdfs:isDefinedBy <http://sibils.org/rdf> ;
      .

:TextPositionSelector
      rdf:type owl:Class ;
      rdfs:label "Text position selector"^^xsd:string ;
      rdfs:comment "A range ot text in a discourse element defined by a start and end position."^^xsd:string ;
      rdfs:subClassOf :oa:TextPositionSelector ;
      rdfs:isDefinedBy <http://sibils.org/rdf> ;
      .

:hasAnnotation a rdf:Property, owl:ObjectProperty ;
      rdfs:label "has annotation"^^xsd:string ;
      rdfs:comment "Links a publication to an annotation generated by named entity extraction."^^xsd:string ;
      rdfs:domain :Publication ;
      rdfs:range :Annotation ;
      rdfs:isDefinedBy <http://sibils.org/rdf> ;
      .

:start a rdf:Property, owl:DatatypeProperty ;
      rdfs:label "start"^^xsd:string ;
      rdfs:comment "Position of the first character of a range of text in a discourse element."^^xsd:string ;
      rdfs:domain :TextPositionSelector ;
      rdfs:range xsd:integer ;
      rdfs:isDefinedBy <http://sibils.org/rdf> ;
      .

:end a rdf:Property, owl:DatatypeProperty ;
      rdfs:label "end"^^xsd:string ;
      rdfs:comment "Position of the last character of a range of text in a discourse element."^^xsd:string ;
      rdfs:domain :TextPositionSelector ;
      rdfs:range xsd:integer ;
      rdfs:isDefinedBy <http://sibils.org/rdf> ;
      .

:exact a rdf:Property, owl:DatatypeProperty ;
      rdfs:label "end"^^xsd:string ;
      rdfs:comment "Text representing the annotated concept as found in the discourse element."^^xsd:string ;
      rdfs:domain :TextPositionSelector ;
      rdfs:range xsd:string ;
      rdfs:isDefinedBy <http://sibils.org/rdf> ;
      .

:hasBody a rdf:Property, owl:ObjectProperty ;
      rdfs:label "has body"^^xsd:string ;
      rdfs:comment "Annotation body. The property object is a concept."^^xsd:string ;
      rdfs:domain :Annotation ;
      rdfs:range skos:Concept ;
      rdfs:isDefinedBy <http://sibils.org/rdf> ;
      .


:hasSelector a rdf:Property, owl:ObjectProperty ;
      rdfs:label "has selector"^^xsd:string ;
      rdfs:comment "Annotation selector. The property object is a selector defining a range of text in a discourse element."^^xsd:string ;
      rdfs:domain :AnnotationTarget ;
      rdfs:range :TextPositionSelector ;
      rdfs:isDefinedBy <http://sibils.org/rdf> ;
      .

:hasSource a rdf:Property, owl:ObjectProperty ;
      rdfs:label "has source"^^xsd:string ;
      rdfs:comment "Source of the annotation. The property object is a discourse element."^^xsd:string ;
      rdfs:domain :AnnotationTarget ;
      rdfs:range :DiscourseElement ;
      rdfs:isDefinedBy <http://sibils.org/rdf> ;
      .

:hasTarget a rdf:Property, owl:ObjectProperty ;
      rdfs:label "has target"^^xsd:string ;
      rdfs:comment "Annotation target. The property object defines the positional coordinates of the annotation concept in a discourse element."^^xsd:string ;
      rdfs:domain :Annotation ;
      rdfs:range :AnnotationTarget ;
      rdfs:isDefinedBy <http://sibils.org/rdf> ;
      .


# Classes and properties derived from cnt http://www.w3.org/2011/content#

:chars a rdf:Property, owl:ObjectProperty ;
      rdfs:label "chars"^^xsd:string ;
      rdfs:comment "The character sequence of a discourse element."^^xsd:string ;
      rdfs:domain :DiscourseElement ;
      rdfs:range xsd:string ;
      rdfs:isDefinedBy <http://sibils.org/rdf> ;
      .





